Documentation.

src/dafny/smart/MerkleTrees.dfy
@@ -13,7 +13,7 @@
  */
 
 include "Helpers.dfy"
-include "Trees.dfy"
+include "Trees2.dfy"
 
 module MerkleTrees {
 
@@ -26,19 +26,36 @@ module MerkleTrees {
      *  @param  root    A tree.
      *  @param  default The default vakue for right-padding the tree leaves.
      *
-     *  We assume collectLeaves return an indexed from left to right list of leaves.
+     *  We assume leavesIn return an indexed from left to right list of leaves.
      *
      *  @todo           We can use another function that returns the values instead
      *                  of collectleaves (returns the seq of values directly) and then
      *                  no need for `x.v`.
      */
-    predicate treeLeftmostLeavesMatchList<T>(l: seq<T>, root: Tree<T>, default: T)
-        requires |l| <= |collectLeaves(root)|
+    predicate treeLeftmostLeavesMatchList<T>(l: seq<T>, root: ITree<T>, default: T)
+        requires |l| <= |leavesIn(root)|
     {
         forall i:: 
-            (0 <= i < |l| ==> l[i] == collectLeaves(root)[i].v)
+            (0 <= i < |l| ==> l[i] == leavesIn(root)[i].v)
             && 
-            (|l| <= i < |collectLeaves(root)|  ==> collectLeaves(root)[i].v == default)
+            (|l| <= i < |leavesIn(root)|  ==> leavesIn(root)[i].v == default)
+    }
+
+    /**
+     *  Whether the tree is a Merkle Tree.
+     *
+     *  The tree must be:
+     *      1.  complete
+     *      2.  the first |l| leftmost leaves hold the values of `l`
+     *      3.  the values on the internal nodes correspond to the value of
+     *          synthesied attribute `f`.
+     */
+    predicate isMerkle<T>(root: ITree<T>, l: seq<T>, f : (T, T) -> T, default: T) 
+        requires |l| <= |leavesIn(root)|
+    {
+        isCompleteTree(root)
+        && isDecoratedWith(f, root)
+        && treeLeftmostLeavesMatchList(l, root, default)
     }
 
     /**
@@ -46,25 +63,25 @@ module MerkleTrees {
      */
     // function default<T>() : T 
 
-    /**
-     *  Check that a decorated tree correctly stores the f attribute. 
-     */
-    predicate isDecoratedWith<T>(f : (T, T) -> T, root: Tree<T>)
-        decreases root
-    {
-        match root
+    // /**
+    //  *  Check that a decorated tree correctly stores the f attribute. 
+    //  */
+    // predicate isDecoratedWith<T>(f : (T, T) -> T, root: ITree<T>)
+    //     decreases root
+    // {
+    //     match root
 
-            case Leaf(v) => 
-                    //  leaves define the attributes
-                    true
+    //         case Leaf(v) => 
+    //                 //  leaves define the attributes
+    //                 true
 
-            case Node(v, lc, rc) => 
-                    //  Recursive definition for an internal node: children are
-                    //  well decorated and node value if the f between children.
-                    v == f(lc.v, rc.v)
-                    && isDecoratedWith(f, lc)
-                    && isDecoratedWith(f, rc)
-    }
+    //         case Node(v, lc, rc) => 
+    //                 //  Recursive definition for an internal node: children are
+    //                 //  well decorated and node value if the f between children.
+    //                 v == f(lc.v, rc.v)
+    //                 && isDecoratedWith(f, lc)
+    //                 && isDecoratedWith(f, rc)
+    // }
 
    /** 
     *  Defines the Tree associated with a given sequence.
@@ -78,33 +95,33 @@ module MerkleTrees {
     *   @param  f   A function to combine two values.
     *   @param  d   A default value for the leaves not in `l`.
     */
-    function buildMerkle<T>(l: seq<T>, h : nat, f : (T, T) -> T, d : T) : Tree<T> 
-        requires h >= 1
-        /** Tree has enough leaves to store `l`. */
-        requires |l| <= power2(h - 1)      
+    // function buildMerkle<T>(l: seq<T>, h : nat, f : (T, T) -> T, d : T) : ITree<T> 
+    //     requires h >= 1
+    //     /** Tree has enough leaves to store `l`. */
+    //     requires |l| <= power2(h - 1)      
 
-        ensures height(buildMerkle(l, h, f, d)) == h
-        ensures isCompleteTree(buildMerkle(l, h, f, d))
-        ensures |collectLeaves(buildMerkle(l, h, f, d))| == power2(h - 1)
-        ensures isDecoratedWith(f, buildMerkle(l, h, f, d))
-        ensures treeLeftmostLeavesMatchList(l, buildMerkle(l, h, f, d), d)
+    //     ensures height(buildMerkle(l, h, f, d)) == h
+    //     ensures isCompleteTree(buildMerkle(l, h, f, d))
+    //     ensures |leavesIn(buildMerkle(l, h, f, d))| == power2(h - 1)
+    //     ensures isDecoratedWith(f, buildMerkle(l, h, f, d))
+    //     ensures treeLeftmostLeavesMatchList(l, buildMerkle(l, h, f, d), d)
 
-        /**
-         *  The tree decorated with constant values.
-         *  
-         *  @param  r   A tree.
-         *  @param  c   A value.
-         *  @returns    True if and olny if all values are equal to `c`.
-         */
-        predicate isConstantTree<T>(r : Tree<T>, c: T) 
-            decreases r
-        {
-            match r 
-                case Leaf(v) => v == c
-                case Node(v, lc, rc) => v == c
-                                && isConstantTree(lc, c) 
-                                && isConstantTree(rc, c)
-        }
+    // /**
+    //     *  The tree decorated with constant values.
+    //     *  
+    //     *  @param  r   A tree.
+    //     *  @param  c   A value.
+    //     *  @returns    True if and olny if all values are equal to `c`.
+    //     */
+    // predicate isConstantITree<T>(r : ITree<T>, c: T) 
+    //     decreases r
+    // {
+    //     match r 
+    //         case ILeaf(v,_) => v == c
+    //         case INode(v, lc, rc,_) => v == c
+    //                         && isConstantITree(lc, c) 
+    //                         && isConstantITree(rc, c)
+    // }
 
     //  Helpers lemmas
 
